AwsCryptographicMaterialProviders/dafny/AwsCryptographyKeyStoreAdmin/src/SystemKey.dfy
@@ -1,0 +1,255 @@
+// Copyright Amazon.com Inc. or its affiliates. All Rights Reserved.
+// SPDX-License-Identifier: Apache-2.0
+include "../Model/AwsCryptographyKeyStoreAdminTypes.dfy"
+include "KmsUtils.dfy"
+include "../../../dafny/AwsCryptographicMaterialProviders/src/CanonicalEncryptionContext.dfy"
+include "../../../dafny/AwsCryptographicMaterialProviders/src/Index.dfy"
+include "../../../dafny/AwsCryptographicMaterialProviders/src/Keyrings/AwsKms/AwsKmsUtils.dfy"
+
+module {:options "/functionSyntax:4" } SystemKey {
+  import opened Wrappers
+  import opened StandardLibrary.UInt
+  import KMS = Com.Amazonaws.Kms
+  import Types = AwsCryptographyKeyStoreAdminTypes
+  import KmsUtils
+  import AtomicPrimitives
+  import CanonicalEncryptionContext
+  import MPL = MaterialProviders
+  import Base64
+  import UTF8
+  import AwsKmsUtils
+  import Structure
+
+  // https://cyberchef.infosec.amazon.dev/#recipe=Encode_text('UTF-8%20(65001)')To_Decimal('Comma',false)&input=ZGlnZXN0&oenc=65001&oeol=CR
+  const DIGEST_UTF8_BYTES: seq<uint8> := [100,105,103,101,115,116]
+  // https://cyberchef.infosec.amazon.dev/#recipe=Encode_text('UTF-8%20(65001)')To_Decimal('Comma',false)&input=c2lnbg&oenc=65001&oeol=CR
+  const SIGN_UTF8_BYTES: seq<uint8> := [115,105,103,110]
+
+  lemma UTF8BytesAreValid()
+    ensures
+      && UTF8.IsASCIIString("digest")
+      && UTF8.EncodeAscii("digest") == DIGEST_UTF8_BYTES
+      ==> UTF8.ValidUTF8Seq(DIGEST_UTF8_BYTES)
+    ensures
+      && UTF8.IsASCIIString("sign")
+      && UTF8.EncodeAscii("sign") == SIGN_UTF8_BYTES
+      ==> UTF8.ValidUTF8Seq(SIGN_UTF8_BYTES)
+  {}
+
+  type SignError = e: Types.Error | (e.KeyStoreAdminException? || e.ComAmazonawsKms?) witness *
+  type VerifyError = e: Types.Error | (e.KeyStoreAdminException? || e.ComAmazonawsKms? || e.MutationVerificationException?) witness *
+  type SerializeError =  e: Types.Error | e. KeyStoreAdminException? witness *
+
+  datatype Content = | Content(
+    nameonly ContentToSHA: MPL.Types.EncryptionContext,
+    nameonly PartionValue: string,
+    nameonly SortValue: string,
+    nameonly UUIDValue: string
+  )
+  {
+    ghost predicate ValidState()
+    {
+      && 0 < |ContentToSHA|
+      && 0 < |PartionValue|
+      && 0 < |SortValue|
+      && 0 < |UUIDValue|
+    }
+  }
+
+  datatype SignInput = | SignInput (
+    nameonly MaterialIdentifier: KMS.Types.KeyIdType,
+    nameonly Content: Content,
+    nameonly KmsTuple: KmsUtils.KMSTuple,
+    nameonly Crypto: AtomicPrimitives.AtomicPrimitivesClient
+  )
+  {
+    ghost predicate ValidState()
+    {
+      && KmsTuple.ValidState()
+      && Crypto.ValidState()
+      && Content.ValidState()
+    }
+  }
+
+  datatype VerifyInput = | VerifyInput (
+    nameonly MaterialIdentifier: KMS.Types.KeyIdType,
+    nameonly Content: Content,
+    nameonly CiphertextBlob: KMS.Types.CiphertextType,
+    nameonly KmsTuple: KmsUtils.KMSTuple,
+    nameonly Crypto: AtomicPrimitives.AtomicPrimitivesClient
+  )
+  {
+    ghost predicate ValidState()
+    {
+      && KmsTuple.ValidState()
+      && Crypto.ValidState()
+      && Content.ValidState()
+    }
+  }
+
+  method ProvideCryptoClient(
+    // Crypto?: Option<AtomicPrimitives.Types.IAwsCryptographicPrimitivesClient> := None
+    Crypto?: Option<AtomicPrimitives.AtomicPrimitivesClient> := None
+  )
+    returns (output: Result<AtomicPrimitives.AtomicPrimitivesClient, AtomicPrimitives.Types.Error>)
+    requires Crypto?.Some? ==> Crypto?.value.ValidState()
+    modifies (if Crypto?.Some? then Crypto?.value.Modifies else {})
+    ensures output.Success?
+            ==>
+              && output.value.ValidState()
+              && fresh(output.value)
+              && fresh(output.value.Modifies)
+  {
+    var Crypto: AtomicPrimitives.AtomicPrimitivesClient; //AtomicPrimitives.Types.IAwsCryptographicPrimitivesClient;
+    if (Crypto?.None?) {
+      Crypto :- AtomicPrimitives.AtomicPrimitives();
+    } else {
+      Crypto := Crypto?.value;
+    }
+    // If the customer gave us the Crypto Client, it is fresh
+    // If we create the Crypto Client, it is fresh
+    assume {:axiom} fresh(Crypto) && fresh(Crypto.Modifies);
+    return Success(Crypto);
+  }
+
+  method SignContent(
+    input: SignInput
+  )
+    returns (output: Result<KMS.Types.CiphertextType, SignError>)
+    requires input.ValidState()
+    ensures input.ValidState()
+    modifies input.KmsTuple.Modifies
+    modifies input.Crypto.Modifies
+  {
+    // =- 1. EncryptionContextDigest
+    // =- 2. Base64 Encode
+    // =- 3.a Base64 encoded content in EC, along with parition key and sort key
+    var kms_ec: KMS.Types.EncryptionContextType :- ContentToKmsEncryptionContext(
+      input.Content,
+      input.Crypto);
+    hide *;
+    // =- 3.b "Sign" as the plaintext
+    var kmsReq := KMS.Types.EncryptRequest(
+      KeyId := input.MaterialIdentifier,
+      // KMS Plaintext type is Blob, so UTF8 Bytes is fine
+      Plaintext := SIGN_UTF8_BYTES,
+      EncryptionContext := Some(kms_ec),
+      GrantTokens := Some(input.KmsTuple.grantTokens)
+    );
+    var kmsRes? := input.KmsTuple.kmsClient.Encrypt(kmsReq);
+    // TODO-Mutations-GA : better error message for failure
+    var kmsRes :- kmsRes?.MapFailure(e => Types.ComAmazonawsKms(e));
+    :- Need(
+      kmsRes.CiphertextBlob.Some?,
+      // TODO-Mutations-GA : better error message for failure
+      Types.KeyStoreAdminException(message := "KMS returned an invalid response.")
+    );
+    // =- 4. return KMS cipher-text result
+    return Success(kmsRes.CiphertextBlob.value);
+  }
+
+  method VerifyContent(
+    input: VerifyInput
+  )
+    returns (output: Result<bool, VerifyError>)
+    requires input.ValidState()
+    ensures input.ValidState()
+    modifies input.KmsTuple.Modifies
+    modifies input.Crypto.Modifies
+  {
+    // =- 1. EncryptionContextDigest
+    // =- 2. Base64 Encode
+    // =- 3.a Base64 encoded content in EC, along with parition key and sort key
+    var kms_ec: KMS.Types.EncryptionContextType :- ContentToKmsEncryptionContext(
+      input.Content,
+      input.Crypto);
+    hide *;
+    var kmsReq := KMS.Types.DecryptRequest(
+      KeyId := Some(input.MaterialIdentifier),
+      CiphertextBlob := input.CiphertextBlob,
+      EncryptionContext := Some(kms_ec),
+      GrantTokens := Some(input.KmsTuple.grantTokens)
+    );
+    var kmsRes? := input.KmsTuple.kmsClient.Decrypt(kmsReq);
+    // TODO-Mutations-GA : better error message for failure
+    // Particularly, if the error is InvalidCiphertextException
+    // than the content has been tampered with
+    // and we should return  MutationVerificationException.
+    // Otherwise, it is some other KMS issue, and we return a KeyStoreAdminException
+    var kmsRes :- kmsRes?.MapFailure(e => Types.ComAmazonawsKms(e));
+    :- Need(
+      kmsRes.Plaintext.Some?,
+      // TODO-Mutations-GA : better error message for failure
+      Types.KeyStoreAdminException(message := "KMS returned an invalid response.")
+    );
+    // =- 4. Assert plain-text is "Sign"
+    :- Need(
+      kmsRes.Plaintext.value == SIGN_UTF8_BYTES,
+      // TODO-Mutations-GA : better error message for failure
+      Types.KeyStoreAdminException(message := "KMS returned an invalid response.")
+    );
+    return Success(true);
+
+  }
+
+  method {:vcs_split_on_every_assert} ContentToKmsEncryptionContext(
+    Content: Content,
+    Crypto: AtomicPrimitives.AtomicPrimitivesClient
+  )
+    returns (output: Result<KMS.Types.EncryptionContextType, SerializeError>)
+    requires Crypto.ValidState() && Content.ValidState()
+    ensures Crypto.ValidState()
+    modifies Crypto.Modifies
+    ensures output.Failure? ==> output.error.KeyStoreAdminException?
+  {
+    hide *;
+    //=- 1. EncryptionContextDigest
+    var digestResult: Result<seq<uint8>, CanonicalEncryptionContext.CanonizeDigestError> :=
+      CanonicalEncryptionContext.EncryptionContextDigest(Crypto, Content.ContentToSHA);
+    if (digestResult.Failure?) {
+      var error: Types.Error;
+      error := match digestResult.error {
+        case AwsCryptographyPrimitives(e) =>
+          // we cannot reliably serialize a Primitive error without work
+          Types.KeyStoreAdminException(message:="Could not SHA-384 Content.")
+        case AwsCryptographicMaterialProvidersException(e) =>
+          Types.KeyStoreAdminException(message:="Could not SHA-384 Content. " + e)
+      };
+      return Failure(error);
+    }
+    //=- 2. Base64 Encode
+    var encodeResult: Result<MPL.Types.Utf8Bytes, string> :=
+      UTF8.Encode(Base64.Encode(digestResult.value));
+    if (encodeResult.Failure?) {
+      var error := Types.KeyStoreAdminException(
+        message:="Could not serialize Digest of content. " + encodeResult.error
+      );
+      return Failure(error);
+    }
+    //=- 3. Base64 encoded content in EC, along with parition key and sort key
+    // Dafny forgets that DIGEST_UTF8_BYTES is valid
+    assert UTF8.ValidUTF8Seq(DIGEST_UTF8_BYTES) by {
+      UTF8BytesAreValid();
+      // TODO-Mutations-FF : What do we need to do convince Dafny this is true?
+      assume {:axiom} UTF8.ValidUTF8Seq(DIGEST_UTF8_BYTES);
+    }
+    var ec_utf8 := map[DIGEST_UTF8_BYTES := encodeResult.value];
+    // Dafny forgets that DIGEST_UTF8_BYTES is valid and all the other keys are valid.
+    assert forall k | k in ec_utf8.Keys :: UTF8.ValidUTF8Seq(k);
+    //=- 4. Stringify Content for KMS
+    var ecResult: Result<KMS.Types.EncryptionContextType, AwsKmsUtils.StringifyError> :=
+      AwsKmsUtils.StringifyEncryptionContext(ec_utf8);
+    if (ecResult.Failure?) {
+      // Right now, all the Errors from the MPL's StringifyEncryptionContext are the MPL error
+      var error := Types.KeyStoreAdminException(message := ecResult.error.message);
+      return Failure(error);
+    }
+    var rtn: KMS.Types.EncryptionContextType := ecResult.value
+    + map[
+      Structure.M_UUID := Content.UUIDValue,
+      Structure.BRANCH_KEY_IDENTIFIER_FIELD := Content.PartionValue,
+      Structure.TYPE_FIELD := Content.SortValue
+    ];
+    return Success(rtn);
+  }
+}
